# The fusc function -- Part 1

##Â Description

The fusc function is defined recursively as follows:

```python
1. fusc(0) = 0
2. fusc(1) = 1
3. fusc(2 * n) = fusc(n)
4. fusc(2 * n + 1) = fusc(n) + fusc(n + 1)
```

The 4 rules above are sufficient to determine the value of `fusc` for any non-negative input `n`. For example, let's say you want to compute `fusc(10)`.

```python
fusc(10) = fusc(5), by rule 3.
fusc(5) = fusc(2) + fusc(3), by rule 4.
fusc(2) = fusc(1), by rule 3.
fusc(1) = 1, by rule 2.
fusc(3) = fusc(1) + fusc(2) by rule 4.
fusc(1) and fusc(2) have already been computed are both equal to 1.
```

Putting these results together `fusc(10) = fusc(5) = fusc(2) + fusc(3) = 1 + 2 = 3`

Your job is to produce the code for the `fusc` function. In this kata, your function will be tested with small values of `n`, so you should not need to be concerned about stack overflow or timeouts.

_Hint: Use recursion._
